chore: drop parentheses

RISCV/SailPure.lean
@@ -8,6 +8,6 @@ open LeanRV64D.Functions
 
 namespace SailRV64I
 
-def addiw (imm : (BitVec 12)) (rs1_val : (BitVec 64)) : BitVec 64 :=
+def addiw (imm : BitVec 12) (rs1_val : BitVec 64) : BitVec 64 :=
   let result :=  rs1_val + (sign_extend (m := ((2 ^i 3) *i 8)) imm)
   (sign_extend (m := ((2 ^i 3) *i 8)) (Sail.BitVec.extractLsb result 31 0))
