RISCV/SailPureToInstructions.lean
@@ -8,7 +8,7 @@ import RISCV.Instructions
 
 namespace RV64I
 
-theorem add_eq (imm : (BitVec 12)) (rs1_val : (BitVec 64)) :
+theorem add_eq (imm : BitVec 12) (rs1_val : BitVec 64) :
     SailRV64I.addiw imm rs1_val = RV64I.addiw imm rs1_val := by
   simp only [SailRV64I.addiw, LeanRV64D.Functions.sign_extend, Sail.BitVec.signExtend, Nat.sub_zero,
     Nat.reduceAdd, Sail.BitVec.extractLsb, RV64I.addiw, BitVec.add_eq]
