RISCV/SailToRV64.lean
@@ -8,5 +8,5 @@ import RISCV.Skeleton
 open LeanRV64D.Functions
 
 theorem add_eq (imm : BitVec 12) (rs1 : regidx) (rd : regidx) :
-    execute_ADDIW (imm) (rs1) (rd) = skeleton_unary rs1 rd (SailRV64I.addiw imm) := by
+    execute_ADDIW  imm rs1 rd = skeleton_unary rs1 rd (SailRV64I.addiw imm) := by
   simp [execute_ADDIW, skeleton_unary, SailRV64I.addiw]
